libcrux-ml-kem/proofs/fstar/extraction/Libcrux_ml_kem.Polynomial.fst
@@ -439,7 +439,7 @@ let subtract_reduce
 
 #pop-options
 
-#push-options "--admit_smt_queries true"
+#push-options "--z3rlimit 300 --split_queries always"
 
 let add_message_error_reduce
       (#v_Vector: Type0)
@@ -448,35 +448,83 @@ let add_message_error_reduce
           Libcrux_ml_kem.Vector.Traits.t_Operations v_Vector)
       (myself message result: t_PolynomialRingElement v_Vector)
      =
+  let e_result:t_Array v_Vector (mk_usize 16) = result.f_coefficients in
   let result:t_PolynomialRingElement v_Vector =
     Rust_primitives.Hax.Folds.fold_range (mk_usize 0)
       v_VECTORS_IN_RING_ELEMENT
-      (fun result temp_1_ ->
+      (fun result i ->
           let result:t_PolynomialRingElement v_Vector = result in
-          let _:usize = temp_1_ in
-          true)
+          let i:usize = i in
+          (forall j. j < v i ==> is_bounded_vector 3328 result.f_coefficients.[ sz j ]) /\
+          (forall j. (j >= v i /\ j < 16) ==> result.f_coefficients.[ sz j ] == e_result.[ sz j ]))
       result
       (fun result i ->
           let result:t_PolynomialRingElement v_Vector = result in
           let i:usize = i in
+          let _:Prims.unit =
+            assert (v i < 16);
+            Spec.Utils.pow2_values_more 15;
+            assert_norm (1441 < pow2 15);
+            assert_norm (1664 < pow2 15);
+            assert_norm (mk_i16 1441 <. mk_i16 1664);
+            assert (Spec.Utils.is_i16b 1664 (mk_i16 1441))
+          in
           let coefficient_normal_form:v_Vector =
             Libcrux_ml_kem.Vector.Traits.f_montgomery_multiply_by_constant #v_Vector
               #FStar.Tactics.Typeclasses.solve
               (result.f_coefficients.[ i ] <: v_Vector)
               (mk_i16 1441)
           in
-          let tmp:v_Vector =
+          let _:Prims.unit =
+            Spec.Utils.lemma_add_intb_forall 3328 3328;
+            assert (6656 <= (pow2 15 - 1));
+            Spec.Utils.lemma_intb_le 6656 (pow2 15 - 1);
+            assert (forall j.
+                  Spec.Utils.is_intb 6656
+                    (v (Seq.index (i1.f_to_i16_array myself.f_coefficients.[ i ]) j) +
+                      v (Seq.index (i1.f_to_i16_array message.f_coefficients.[ i ]) j)));
+            assert (forall j.
+                  Spec.Utils.is_intb (pow2 15 - 1)
+                    (v (Seq.index (i1.f_to_i16_array myself.f_coefficients.[ i ]) j) +
+                      v (Seq.index (i1.f_to_i16_array message.f_coefficients.[ i ]) j)))
+          in
+          let sum1:v_Vector =
             Libcrux_ml_kem.Vector.Traits.f_add #v_Vector
               #FStar.Tactics.Typeclasses.solve
               (myself.f_coefficients.[ i ] <: v_Vector)
               (message.f_coefficients.[ i ] <: v_Vector)
           in
-          let tmp:v_Vector =
+          let _:Prims.unit = assert (is_bounded_vector 6656 sum1) in
+          let _:Prims.unit =
+            Spec.Utils.lemma_add_intb_forall 3328 6656;
+            Spec.Utils.lemma_intb_le 9984 (pow2 15 - 1);
+            Spec.Utils.lemma_intb_le 9984 28296;
+            assert (forall j.
+                  Spec.Utils.is_intb 9984
+                    (v (Seq.index (i1.f_to_i16_array coefficient_normal_form) j) +
+                      v (Seq.index (i1.f_to_i16_array sum1) j)));
+            assert (forall j.
+                  Spec.Utils.is_intb 28296
+                    (v (Seq.index (i1.f_to_i16_array coefficient_normal_form) j) +
+                      v (Seq.index (i1.f_to_i16_array sum1) j)));
+            assert (forall j.
+                  Spec.Utils.is_intb (pow2 15 - 1)
+                    (v (Seq.index (i1.f_to_i16_array coefficient_normal_form) j) +
+                      v (Seq.index (i1.f_to_i16_array sum1) j)))
+          in
+          let sum2:v_Vector =
             Libcrux_ml_kem.Vector.Traits.f_add #v_Vector
               #FStar.Tactics.Typeclasses.solve
               coefficient_normal_form
-              tmp
+              sum1
           in
+          let _:Prims.unit = assert (is_bounded_vector 9984 sum2) in
+          let red:v_Vector =
+            Libcrux_ml_kem.Vector.Traits.f_barrett_reduce #v_Vector
+              #FStar.Tactics.Typeclasses.solve
+              sum2
+          in
+          let _:Prims.unit = assert (is_bounded_vector 3328 red) in
           let result:t_PolynomialRingElement v_Vector =
             {
               result with
@@ -484,14 +532,17 @@ let add_message_error_reduce
               =
               Rust_primitives.Hax.Monomorphized_update_at.update_at_usize result.f_coefficients
                 i
-                (Libcrux_ml_kem.Vector.Traits.f_barrett_reduce #v_Vector
-                    #FStar.Tactics.Typeclasses.solve
-                    tmp
-                  <:
-                  v_Vector)
+                red
             }
             <:
             t_PolynomialRingElement v_Vector
+          in
+          let _:Prims.unit =
+            assert (forall j.
+                  (j > v i /\ j < 16) ==> result.f_coefficients.[ sz j ] == e_result.[ sz j ]);
+            assert (forall j. j < v i ==> is_bounded_vector 3328 result.f_coefficients.[ sz j ]);
+            assert (result.f_coefficients.[ i ] == red);
+            assert (forall j. j <= v i ==> is_bounded_vector 3328 result.f_coefficients.[ sz j ])
           in
           result)
   in
@@ -595,7 +646,7 @@ let to_standard_domain
     vector
     Libcrux_ml_kem.Vector.Traits.v_MONTGOMERY_R_SQUARED_MOD_FIELD_MODULUS
 
-#push-options "--z3rlimit 300"
+#push-options "--z3rlimit 300 --split_queries always"
 
 let add_standard_error_reduce
       (#v_Vector: Type0)
@@ -621,6 +672,7 @@ let add_standard_error_reduce
             to_standard_domain #v_Vector (myself.f_coefficients.[ j ] <: v_Vector)
           in
           let _:Prims.unit =
+            Spec.Utils.pow2_values_more 15;
             assert (is_bounded_vector 3328 coefficient_normal_form);
             assert (is_bounded_vector 3328 (error.f_coefficients.[ j ]));
             Spec.Utils.lemma_add_intb_forall 3328 3328;
@@ -678,7 +730,7 @@ let add_standard_error_reduce
 
 #pop-options
 
-#push-options "--admit_smt_queries true"
+#push-options "--z3rlimit 300"
 
 let ntt_multiply
       (#v_Vector: Type0)
@@ -753,22 +805,6 @@ let impl_2__ZERO
   }
   <:
   t_PolynomialRingElement v_Vector
-
-let impl_2__add_message_error_reduce
-      (#v_Vector: Type0)
-      (#[FStar.Tactics.Typeclasses.tcresolve ()]
-          i1:
-          Libcrux_ml_kem.Vector.Traits.t_Operations v_Vector)
-      (self message result: t_PolynomialRingElement v_Vector)
-     = add_message_error_reduce #v_Vector self message result
-
-let impl_2__ntt_multiply
-      (#v_Vector: Type0)
-      (#[FStar.Tactics.Typeclasses.tcresolve ()]
-          i1:
-          Libcrux_ml_kem.Vector.Traits.t_Operations v_Vector)
-      (self rhs: t_PolynomialRingElement v_Vector)
-     = ntt_multiply #v_Vector self rhs
 
 let impl_2__num_bytes
       (#v_Vector: Type0)
@@ -933,6 +969,14 @@ let impl_2__subtract_reduce
       (self b: t_PolynomialRingElement v_Vector)
      = subtract_reduce #v_Vector self b
 
+let impl_2__add_message_error_reduce
+      (#v_Vector: Type0)
+      (#[FStar.Tactics.Typeclasses.tcresolve ()]
+          i1:
+          Libcrux_ml_kem.Vector.Traits.t_Operations v_Vector)
+      (self message result: t_PolynomialRingElement v_Vector)
+     = add_message_error_reduce #v_Vector self message result
+
 let impl_2__add_error_reduce
       (#v_Vector: Type0)
       (#[FStar.Tactics.Typeclasses.tcresolve ()]
@@ -952,3 +996,11 @@ let impl_2__add_standard_error_reduce
      =
   let self:t_PolynomialRingElement v_Vector = add_standard_error_reduce #v_Vector self error in
   self
+
+let impl_2__ntt_multiply
+      (#v_Vector: Type0)
+      (#[FStar.Tactics.Typeclasses.tcresolve ()]
+          i1:
+          Libcrux_ml_kem.Vector.Traits.t_Operations v_Vector)
+      (self rhs: t_PolynomialRingElement v_Vector)
+     = ntt_multiply #v_Vector self rhs
